crdt_examples.thy
@@ -1,0 +1,148 @@
+theory crdt_examples
+  imports crdt_specs
+begin
+
+section "CRDT Examples"
+
+text \<open>We illustrate the different map semantics based on examples:\<close>
+
+abbreviation "c \<equiv> CallId"
+
+definition "hb r \<equiv> (\<lambda>(x,y). (c x, c y))`  r\<^sup>+"
+
+definition "exampleA \<equiv> \<lparr>
+  calls = [
+    c 0 \<mapsto> Call (DeleteKey 1) default, 
+    c 1 \<mapsto> Call (DeleteKey 1) default,
+    c 2 \<mapsto> Call (NestedOp 1 (Increment 1)) default
+  ],
+  happensBefore = hb {(0,2)}
+\<rparr>"
+
+
+definition "exampleB \<equiv> \<lparr>
+  calls = [
+    c 0 \<mapsto> Call (DeleteKey 1) default, 
+    c 1 \<mapsto> Call (DeleteKey 1) default,
+    c 2 \<mapsto> Call (NestedOp 1 (Increment 1)) default,
+    c 3 \<mapsto> Call (NestedOp 1 (Increment 1)) default
+  ],
+  happensBefore = hb {(0,2), (1,3)}
+\<rparr>"
+
+definition "exampleC \<equiv> \<lparr>
+  calls = [
+    c 0 \<mapsto> Call (NestedOp 1 (Increment 1)) default, 
+    c 1 \<mapsto> Call (NestedOp 1 (Increment 1)) default,
+    c 2 \<mapsto> Call (DeleteKey 1) default
+  ],
+  happensBefore = hb {(0,2)}
+\<rparr>"
+
+definition "exampleD \<equiv> \<lparr>
+  calls = [
+    c 0 \<mapsto> Call (NestedOp 1 (Increment 1)) default, 
+    c 1 \<mapsto> Call (NestedOp 1 (Increment 1)) default,
+    c 2 \<mapsto> Call (DeleteKey 1) default,
+    c 3 \<mapsto> Call (DeleteKey 1) default
+  ],
+  happensBefore = hb {(0,2), (1,3)}
+\<rparr>"
+
+
+definition "dom_subset A m \<equiv> A \<inter> dom m"
+
+lemma dom_subset_empty[simp]: "dom_subset {} m = {}"
+  by (simp add: dom_subset_def)
+
+lemma dom_subset_insert[simp]: "dom_subset (insert x A) m = (case m x of Some y \<Rightarrow> {x} | None \<Rightarrow> {}) \<union> dom_subset A m"
+  by (auto simp add: dom_subset_def split: option.splits)
+
+lemma dom_subset_ex:
+  assumes "\<And>x y. m x \<triangleq> y \<Longrightarrow>  x \<in> {c 0, c 1, c 2, c 3}"
+  shows "dom m = dom_subset {c 0, c 1, c 2, c 3} m"
+  using assms by (auto simp add: dom_subset_def)
+
+method eval_example_auto = (auto simp add: map_dw_spec_def map_spec_def
+    counter_spec_def sub_context_def restrict_ctxt_op_def
+    restrict_ctxt_def fmap_map_values_def ctxt_restrict_calls_def
+    restrict_map_def deleted_calls_dw_def 
+    exampleA_def exampleB_def exampleC_def exampleD_def 
+    Op_def hb_def
+    is_update_counterOp_def sum_map_def map_uw_spec_def deleted_calls_uw_def
+    option_bind_def trancl_insert  increments_def nested_op_on_key_def
+    rtrancl_insert
+    map_suw_spec_def deleted_calls_suw_def
+    map_sdw_spec_def deleted_calls_sdw_def
+    split: option.splits if_splits)
+
+method eval_example = (eval_example_auto; (subst dom_subset_ex)?)+
+
+lemma "map_uw_spec counter_spec (NestedOp 1 GetCount) exampleA (from_int 1)"
+  by eval_example
+
+lemma "map_suw_spec counter_spec (NestedOp 1 GetCount) exampleA (from_int 1)"
+  by eval_example
+
+lemma "map_dw_spec counter_spec (NestedOp 1 GetCount) exampleA (from_int 0)"
+  by eval_example
+
+lemma "map_sdw_spec counter_spec (NestedOp 1 GetCount) exampleA (from_int 0)"
+  by eval_example
+    (metis callId.inject)
+
+
+lemma "map_uw_spec counter_spec (NestedOp 1 GetCount) exampleB (from_int 2)"
+  by eval_example
+
+lemma "map_suw_spec counter_spec (NestedOp 1 GetCount) exampleB (from_int 2)"
+  by eval_example
+
+lemma "map_dw_spec counter_spec (NestedOp 1 GetCount) exampleB (from_int 2)"
+  by eval_example
+
+lemma "map_sdw_spec counter_spec (NestedOp 1 GetCount) exampleB (from_int 0)"
+  by eval_example
+    (metis callId.inject)
+
+
+
+
+lemma "map_uw_spec counter_spec (NestedOp 1 GetCount) exampleC (from_int 1)"
+  by eval_example
+
+lemma "map_suw_spec counter_spec (NestedOp 1 GetCount) exampleC (from_int 2)"
+  by eval_example
+    (smt callId.inject)
+
+
+lemma "map_dw_spec counter_spec (NestedOp 1 GetCount) exampleC (from_int 0)"
+  by eval_example
+
+lemma "map_sdw_spec counter_spec (NestedOp 1 GetCount) exampleC (from_int 0)"
+  by eval_example
+    (smt callId.inject)+
+
+
+
+lemma "map_uw_spec counter_spec (NestedOp 1 GetCount) exampleD (from_int 0)"
+  by eval_example
+    (smt callId.inject)
+
+lemma "map_suw_spec counter_spec (NestedOp 1 GetCount) exampleD (from_int 2)"
+  by eval_example
+    (smt callId.inject)
+
+
+lemma "map_dw_spec counter_spec (NestedOp 1 GetCount) exampleD (from_int 0)"
+  by eval_example
+    (smt callId.inject)+
+
+lemma "map_sdw_spec counter_spec (NestedOp 1 GetCount) exampleD (from_int 0)"
+  by eval_example
+    (smt callId.inject)+
+
+
+
+
+end
