extra.thy
@@ -1,0 +1,59 @@
+theory extra
+imports crdt_specs
+begin
+
+section \<open>Extra Material\<close>
+
+text \<open>Some checks for the text.\<close>
+
+lemma set_rw_spec_Contains:
+(*and "trans (happensBefore ctxt)"
+   and "irrefl (happensBefore ctxt)"
+   and "Field (happensBefore ctxt) \<subseteq> dom (calls ctxt)"
+   and "finite (dom (calls ctxt))" *)
+  shows "\<exists>(ctxt::('a setOp, 'b::{from_bool}) operationContext) res.
+set_rw_spec (Contains x) ctxt res
+\<and>  res \<noteq> from_bool ((\<exists>a. Op ctxt a \<triangleq> Add x)
+                           \<and> (\<forall>r. Op ctxt r \<triangleq> Remove x
+                                \<longrightarrow> (\<exists>a. Op ctxt a \<triangleq> Add x
+                                 \<and> (r,a)\<in>happensBefore ctxt)))"
+proof -
+  define ctxt :: "('a setOp, 'b) operationContext" where 
+    "ctxt = \<lparr>calls = (\<lambda>c. Some (Call (Add x) ???)),
+    happensBefore = {(CallId x, CallId y) | x y. x < y}\<rparr>"
+
+  show ?thesis
+  proof (intro exI conjI)
+
+    show "set_rw_spec (Contains x) ctxt (from_bool False)"
+    proof (auto simp add: set_rw_spec_def set_spec_def flag_dw_spec_def intro!: arg_cong[where f=from_bool])
+      assume "Enable \<in> latestOps (restrict_ctxt_op (set_to_flag x) ctxt)"
+        and "Disable \<notin> latestOps (restrict_ctxt_op (set_to_flag x) ctxt)"
+      have "latestOps (restrict_ctxt_op (set_to_flag x) ctxt) = {}"
+        apply (auto simp add: latestOps_def restrict_ctxt_op_def restrict_ctxt_def ctxt_def restrict_hb_def Op_def fmap_map_values_def set_to_flag_def restrict_relation_def split: option.splits)
+        by (metis callId.exhaust gt_ex)
+
+      with `Enable \<in> latestOps (restrict_ctxt_op (set_to_flag x) ctxt)`
+      show False
+        by auto
+    qed
+
+    have no_remove: "Op ctxt r \<noteq> Some (Remove x)" for r
+      by (auto simp add: ctxt_def Op_def)
+
+    have "((\<exists>a. Op ctxt a \<triangleq> Add x) \<and>
+        (\<forall>r. Op ctxt r \<triangleq> Remove x \<longrightarrow> (\<exists>a. Op ctxt a \<triangleq> Add x \<and> (r, a) \<in> happensBefore ctxt)))"
+    proof (intro conjI impI allI exI)
+      show "Op ctxt (CallId 0) \<triangleq> Add x"
+        by (simp add: Op_def ctxt_def)
+    qed (simp add: no_remove)+
+
+    thus "from_bool False \<noteq>
+    from_bool
+     ((\<exists>a. Op ctxt a \<triangleq> Add x) \<and>
+      (\<forall>r. Op ctxt r \<triangleq> Remove x \<longrightarrow> (\<exists>a. Op ctxt a \<triangleq> Add x \<and> (r, a) \<in> happensBefore ctxt)))"
+      using from_bool_eq_simp  by auto
+  qed
+qed
+
+end
